upd

coqimp/ext/finaltheorem.v
@@ -1,5 +1,5 @@
 (*+ Final Theorem Proof +*)
-Require Import Coqlib.
+Require Import Coqlib. 
 Require Import Maps.
 
 Require Import Classical_Prop.
@@ -27,6 +27,56 @@ Unset Strict Implicit.
 Open Scope code_scope.
 Open Scope mem_scope.
 
+Inductive n_tau_step {prog : Type} (step : prog -> msg -> prog -> Prop) :
+  Index -> prog -> prog -> Prop :=
+| Zero_tau_step : forall p idx, n_tau_step step idx p p
+| Multi_tau_step : forall (p p' p'' : prog) idx_i idx_j,
+    step p tau p' -> idx_j ⩹ idx_i -> n_tau_step step idx_j p' p'' -> 
+    n_tau_step step idx_i p p''.
+
+Lemma LEtr_emp_n_step_H_progress :
+  forall LP LP' HP ndx idx,
+    n_tau_step LP__ ndx LP LP' -> wp_sim idx LP HP -> idx ⩹ ndx ->
+    (exists HP' HP'', star_step HP__ HP HP' /\ HP__ HP' tau HP'').
+Proof.
+  intros.
+  generalize dependent LP.
+  generalize dependent LP'.
+  generalize dependent HP.
+
+Lemma wp_sim_ensures_refinement' :
+  forall C Cas S pc npc PrimSet HS B idx,
+    C ⊥ Cas -> wp_sim idx (C ⊎ Cas, (S, pc, npc)) (C, PrimSet, HS) ->
+    Etrace LP__ (C ⊎ Cas, (S, pc, npc)) B ->
+    Etrace HP__ (C, PrimSet, HS) B.
+Proof.
+  cofix Hp.
+  intros.
+  destruct B.
+  {
+  }
+  
+(* Whole program simulation ensures refinement *)
+Lemma wp_sim_ensures_refinement :
+  forall C S pc npc Cas PrimSet HS idx,
+    C ⊥ Cas -> wp_sim idx (C ⊎ Cas, (S, pc, npc)) (C, PrimSet, HS) ->
+    Etr_Refinement (C ⊎ Cas, (S, pc, npc)) (C, PrimSet, HS).
+Proof.
+  intros.
+  unfold Etr_Refinement; intros.
+  eapply wp_sim_ensures_refinement'; eauto.
+Qed.
+
+(* Compositionality1 *)
+Lemma compositionality1 :
+  forall Spec C Cas PrimSet S HS pc npc,
+    simImpsPrimSet Spec Cas PrimSet ->
+    wp_stateRel S HS -> HProgSafe (C, PrimSet, HS) ->
+    get_Hs_pcont HS = (pc, npc) -> C ⊥ Cas ->
+    exists idx, wp_sim idx (C ⊎ Cas, (S, pc, npc)) (C, PrimSet, HS).
+Proof.
+Admitted.
+
 (** Logic ensures simulation *)
 Lemma logic_ensures_simulation :
   forall Spec Cas PrimSet,
@@ -41,7 +91,13 @@ Lemma sim_imp_ctx_refinement :
     simImpsPrimSet Spec Cas PrimSet ->
     correct Cas PrimSet.
 Proof.
-  Admitted.
+  intros.
+  unfold correct; intros.
+  lets Ht : compositionality1 __; eauto.
+  eapply Ht in H; eauto.
+  destruct H as [idx H].
+  eapply wp_sim_ensures_refinement; eauto.
+Qed.  
 
 (** Final Theorem *)
 Theorem FinalTheorem : forall Spec Cas PrimSet,
